introducing uniform & binary and changing to cfg based defintions for CNF (only minor changes in uProds & eProds)

Stimpfle/CNF.thy
@@ -32,109 +32,178 @@ lemma upgr_noeProds:
   using assms 
   unfolding uppr_def noeProds_def uppr_rules_def nonUnitProds_def unitProds_def newProds_def by simp
 
+lemma Nts_correct: "A \<notin> Nts P \<Longrightarrow> (\<nexists>S \<alpha>. (S, \<alpha>) \<in> P \<and> (Nt A \<in> {Nt S} \<union> set \<alpha>))"
+  unfolding Nts_def apply (induction rule: nt.induct) apply simp
+  by (metis Un_iff case_prod_conv in_set_conv_decomp insertCI nt.simps(2) nt_append)
+
+lemma not_in_lang: 
+  assumes "S \<notin> Nts P"  
+  shows "Lang P S = {}"
+  using assms Nts_correct 
+  by (metis Lang_def all_not_in_conv deriven_start1 insert_is_Un list.set_intros(1) list.simps(15) mem_Collect_eq rtranclp_power)
+
 (* Chomsky Normal Form *)
 
-definition trans1Tm :: "'n::infinite \<Rightarrow> 't \<Rightarrow> ('n, 't) prods \<Rightarrow> ('n, 't) prods \<Rightarrow> bool" where 
-      "trans1Tm A t P P' \<equiv> (
-    \<exists> l r p s. (l,r) \<in> set P \<and> (r = p@[Tm t]@s) 
-    \<and> (p \<noteq> [] \<or> s \<noteq> []) \<and> (A = fresh P)
-    \<and> (P' = ((removeAll (l,r) P) @ [(A,[Tm t]), (l, p@[Nt A]@s)])))"
+axiomatization fresh :: "('n::infinite,'t) cfg \<Rightarrow> 'n" where
+fresh: "fresh G \<notin> Nts(set (prods G)) \<union> {start G}"
+term L
+abbreviation L :: "('n,'t) cfg \<Rightarrow> 't list set" where
+  "L G \<equiv> Lang (set (prods G)) (start G)"
+
+definition trans1Tm :: "'n::infinite \<Rightarrow> 't \<Rightarrow> ('n, 't) cfg \<Rightarrow> ('n, 't) cfg \<Rightarrow> bool" where 
+      "trans1Tm A t G G' \<equiv> (
+    \<exists> l r p s. (l,r) \<in> set (prods G) \<and> (r = p@[Tm t]@s) 
+    \<and> (p \<noteq> [] \<or> s \<noteq> []) \<and> (A = fresh G)
+    \<and> prods G' = ((removeAll (l,r) (prods G)) @ [(A,[Tm t]), (l, p@[Nt A]@s)]) 
+    \<and> start G' = start G)"
 
 lemma trans1Tm_noeProds:
-  assumes "noeProds (set P)"
-    and "trans1Tm A t P P'"
-  shows "noeProds (set P')"
+  assumes "noeProds (set (prods G))"
+    and "trans1Tm A t G G'"
+  shows "noeProds (set (prods G'))"
   using assms unfolding trans1Tm_def noeProds_def by force
 
 lemma trans1Tm_noUnitProds:
-  assumes "noUnitProds (set P)"
-    and "trans1Tm A t P P'"
-  shows "noUnitProds (set P')"
+  assumes "noUnitProds (set (prods G))"
+    and "trans1Tm A t G G'"
+  shows "noUnitProds (set (prods G'))"
 proof -
-  have 1: "(\<nexists>l A. (l,[Nt A]) \<in> (set P))"
+  have 1: "(\<nexists>l A. (l,[Nt A]) \<in> (set (prods G)))"
     using assms(1) unfolding noUnitProds_def by simp
-  obtain l r p s where "(l,r) \<in> set P \<and> (r = p@[Tm t]@s) \<and> (p \<noteq> [] \<or> s \<noteq> []) 
-      \<and> set P' = ((set P - {(l,r)}) \<union> {(A,[Tm t]), (l, p@[Nt A]@s)})" (is "?lrps")
+  obtain l r p s where "(l,r) \<in> set (prods G) \<and> (r = p@[Tm t]@s) \<and> (p \<noteq> [] \<or> s \<noteq> []) 
+      \<and> set (prods G') = ((set (prods G) - {(l,r)}) \<union> {(A,[Tm t]), (l, p@[Nt A]@s)})" (is "?lrps")
     using assms(2) set_removeAll unfolding trans1Tm_def by force
   hence "\<nexists>l' A'. (l,[Nt A']) \<in> {(A,[Tm t]), (l, p@[Nt A]@s)}" 
     using Cons_eq_append_conv by fastforce
-  hence "\<nexists>l' A'. (l',[Nt A']) \<in> ((set P - {(l,r)}) \<union> {(A,[Tm t]), (l, p@[Nt A]@s)})"
+  hence "\<nexists>l' A'. (l',[Nt A']) \<in> ((set (prods G) - {(l,r)}) \<union> {(A,[Tm t]), (l, p@[Nt A]@s)})"
     using 1 by simp
-  moreover have "set P' = ((set P - {(l,r)}) \<union> {(A,[Tm t]), (l, p@[Nt A]@s)})"
+  moreover have "set (prods G') = ((set (prods G) - {(l,r)}) \<union> {(A,[Tm t]), (l, p@[Nt A]@s)})"
     using \<open>?lrps\<close> by simp
   ultimately show ?thesis unfolding noUnitProds_def by simp
 qed
 
-find_consts "'a set \<Rightarrow> 'b"
 definition prodTms :: "('n,'t) prod \<Rightarrow> nat" where
-  "prodTms p = (if length (snd p) \<le> 1 then 0 else length (filter (isTmnlSym) (snd p)))"
+  "prodTms p \<equiv> (if length (snd p) \<le> 1 then 0 else length (filter (isTmnlSym) (snd p)))"
 
 definition prodNts :: "('n,'t) prod \<Rightarrow> nat" where
-  "prodNts p = (if length (snd p) \<le> 2 then 0 else length (filter (isNonTmnlSym) (snd p)))"
+  "prodNts p \<equiv> (if length (snd p) \<le> 2 then 0 else length (filter (isNonTmnlSym) (snd p)))"
 
 fun badTmsCount :: "('n,'t) prods \<Rightarrow> nat" where
   "badTmsCount [] = 0" |
   "badTmsCount (p#ps) = (prodTms p) + badTmsCount ps"
 
 lemma badTmsCountSet: "(\<forall>p \<in> set P. prodTms p = 0) \<longleftrightarrow> badTmsCount P = 0"
- apply (induction P) by auto
+  by (induction P) auto
 
 fun badNtsCount :: "('n,'t) prods \<Rightarrow> nat" where
   "badNtsCount [] = 0" |
   "badNtsCount (p#ps) = (prodNts p) + badNtsCount ps"
 
 lemma badNtsCountSet: "(\<forall>p \<in> set P. prodNts p = 0) \<longleftrightarrow> badNtsCount P = 0"
- apply (induction P) by auto
+  by (induction P) auto
 
-definition cnf :: "('n,'t) prods \<Rightarrow> bool" where
-  "cnf P = ((badTmsCount P = 0) \<and> (badNtsCount P = 0))"
+definition uniform :: "('n, 't) cfg \<Rightarrow> bool" where
+  "uniform G \<equiv> \<forall>(A, \<alpha>) \<in> set (prods G). (\<nexists>t. Tm t \<in> set \<alpha>) \<or> (\<exists>t. \<alpha> = [Tm t])"
 
-definition trans2Nt :: "'n::infinite \<Rightarrow> 'n \<Rightarrow> 'n \<Rightarrow> ('n,'t) prods \<Rightarrow> ('n,'t) prods \<Rightarrow> bool" where
-      "trans2Nt A B\<^sub>1 B\<^sub>2 P P' \<equiv> (
-    \<exists>l r p s. (l,r) \<in> set P \<and> (r = p@[Nt B\<^sub>1,Nt B\<^sub>2]@s)
-    \<and> (p \<noteq> [] \<or> s \<noteq> []) \<and> (A = fresh P)
-    \<and> (P' = ((removeAll (l,r) P) @ [(A, [Nt B\<^sub>1,Nt B\<^sub>2]), (l, p@[Nt A]@s)])))"
+lemma uniform_badTmsCount: 
+  "uniform G \<longleftrightarrow> badTmsCount (prods G) = 0"
+proof 
+  assume "uniform G" (is "?assm")
+  have "\<forall>p \<in> set (prods G). prodTms p = 0"
+  proof 
+    fix p assume "p \<in> set (prods G)"
+    hence "(\<nexists>t. Tm t \<in> set (snd p)) \<or> (\<exists>t. snd p = [Tm t])"
+      using \<open>?assm\<close> unfolding uniform_def by auto
+    hence "length (snd p) \<le> 1 \<or> (\<nexists>t. Tm t \<in> set (snd p))"
+      by auto
+    hence "length (snd p) \<le> 1 \<or> length (filter (isTmnlSym) (snd p)) = 0"
+      unfolding isTmnlSym_def by (auto simp: filter_empty_conv)
+    thus "prodTms p = 0"
+      unfolding prodTms_def by argo
+   qed
+   thus "badTmsCount (prods G) = 0"
+     using badTmsCountSet by blast
+next 
+  assume "badTmsCount (prods G) = 0" (is "?assm")
+  have "\<forall>p \<in> set (prods G). ((\<nexists>t. Tm t \<in> set (snd p)) \<or> (\<exists>t. snd p = [Tm t]))"
+  proof 
+    fix p assume "p \<in> set (prods G)"
+    hence "prodTms p = 0"
+      using \<open>?assm\<close> badTmsCountSet by blast
+    hence "length (snd p) \<le> 1 \<or> length (filter (isTmnlSym) (snd p)) = 0"
+      unfolding prodTms_def by argo
+    hence "length (snd p) \<le> 1 \<or> (\<nexists>t. Tm t \<in> set (snd p))"
+      unfolding isTmnlSym_def by (auto simp: filter_empty_conv)
+    hence "length (snd p) = 0 \<or> length (snd p) = 1 \<or> (\<nexists>t. Tm t \<in> set (snd p))"
+      using order_neq_le_trans by blast
+    thus "(\<nexists>t. Tm t \<in> set (snd p)) \<or> (\<exists>t. snd p = [Tm t])"
+      by (auto simp: length_Suc_conv)
+  qed
+  thus "uniform G"
+    unfolding uniform_def by auto
+qed
+
+definition binary :: "('n, 't) cfg \<Rightarrow> bool" where
+  "binary G \<equiv> \<forall>(A, \<alpha>) \<in> set (prods G). length \<alpha> \<le> 2"
+
+lemma binary_badNtsCount:
+  assumes "uniform G" "badNtsCount (prods G) = 0"
+  shows "binary G"
+  using assms sorry
+
+definition cnf :: "('n,'t) cfg \<Rightarrow> bool" where
+  "cnf G = ((badTmsCount (prods G) = 0) \<and> (badNtsCount (prods G) = 0))"
+
+lemma cnf_bin_un: "(binary G \<and> uniform G) \<longleftrightarrow> cnf G"
+  unfolding cnf_def using binary_badNtsCount uniform_badTmsCount sorry
+
+definition trans2Nt :: "'n::infinite \<Rightarrow> 'n \<Rightarrow> 'n \<Rightarrow> ('n,'t) cfg \<Rightarrow> ('n,'t) cfg \<Rightarrow> bool" where
+      "trans2Nt A B\<^sub>1 B\<^sub>2 G G' \<equiv> (
+    \<exists>l r p s. (l,r) \<in> set (prods G) \<and> (r = p@[Nt B\<^sub>1,Nt B\<^sub>2]@s)
+    \<and> (p \<noteq> [] \<or> s \<noteq> []) \<and> (A = fresh G)
+    \<and> prods G' = ((removeAll (l,r) (prods G)) @ [(A, [Nt B\<^sub>1,Nt B\<^sub>2]), (l, p@[Nt A]@s)])
+    \<and> start G' = start G)"
 
 lemma trans2Nt_noeProds:
-  assumes "noeProds (set P)"
-    and "trans2Nt A B\<^sub>1 B\<^sub>2 P P'"
-  shows "noeProds (set P')"
+  assumes "noeProds (set (prods G))"
+    and "trans2Nt A B\<^sub>1 B\<^sub>2 G G'"
+  shows "noeProds (set (prods G'))"
   using assms unfolding trans2Nt_def noeProds_def by force
 
 lemma trans2Nt_noUnitProds:
-  assumes "noUnitProds (set P)"
-    and "trans2Nt A B\<^sub>1 B\<^sub>2 P P'"
-  shows "noUnitProds (set P')"
+  assumes "noUnitProds (set (prods G))"
+    and "trans2Nt A B\<^sub>1 B\<^sub>2 G G'"
+  shows "noUnitProds (set (prods G'))"
   proof -
-  have 1: "(\<nexists>l A. (l,[Nt A]) \<in> (set P))"
+  have 1: "(\<nexists>l A. (l,[Nt A]) \<in> (set (prods G)))"
     using assms(1) unfolding noUnitProds_def by simp
-  obtain l r p s where "(l,r) \<in> set P \<and> (r = p@[Nt B\<^sub>1,Nt B\<^sub>2]@s) \<and> (p \<noteq> [] \<or> s \<noteq> []) 
-      \<and> (set P' = ((set P - {(l,r)}) \<union> {(A, [Nt B\<^sub>1,Nt B\<^sub>2]), (l, p@[Nt A]@s)}))" (is "?lrps")
+  obtain l r p s where "(l,r) \<in> set (prods G) \<and> (r = p@[Nt B\<^sub>1,Nt B\<^sub>2]@s) \<and> (p \<noteq> [] \<or> s \<noteq> []) 
+      \<and> (set (prods G') = ((set (prods G) - {(l,r)}) \<union> {(A, [Nt B\<^sub>1,Nt B\<^sub>2]), (l, p@[Nt A]@s)}))" (is "?lrps")
     using assms(2) set_removeAll unfolding trans2Nt_def by force
   hence "\<nexists>l' A'. (l,[Nt A']) \<in> {(A, [Nt B\<^sub>1,Nt B\<^sub>2]), (l, p@[Nt A]@s)}" 
     using Cons_eq_append_conv by fastforce
-  hence "\<nexists>l' A'. (l',[Nt A']) \<in> ((set P - {(l,r)}) \<union> {(A, [Nt B\<^sub>1,Nt B\<^sub>2]), (l, p@[Nt A]@s)})"
+  hence "\<nexists>l' A'. (l',[Nt A']) \<in> ((set (prods G) - {(l,r)}) \<union> {(A, [Nt B\<^sub>1,Nt B\<^sub>2]), (l, p@[Nt A]@s)})"
     using 1 by simp
-  moreover have "set P' = ((set P - {(l,r)}) \<union> {(A, [Nt B\<^sub>1,Nt B\<^sub>2]), (l, p@[Nt A]@s)})"
+  moreover have "set (prods G') = ((set (prods G) - {(l,r)}) \<union> {(A, [Nt B\<^sub>1,Nt B\<^sub>2]), (l, p@[Nt A]@s)})"
     using \<open>?lrps\<close> by simp
   ultimately show ?thesis unfolding noUnitProds_def by simp
 qed
 
 lemma trans2Nt_aux1:
-  assumes "trans2Nt A B\<^sub>1 B\<^sub>2 P P'"
+  assumes "trans2Nt A B\<^sub>1 B\<^sub>2 G G'"
   shows "A \<noteq> B\<^sub>1 \<and> A \<noteq> B\<^sub>2"
   using assms fresh unfolding trans2Nt_def Nts_def by fastforce
 
 
 lemma cnf_r1Tm: 
-  assumes "trans1Tm A t P P'"
-    and "set P \<turnstile> lhs \<Rightarrow> rhs"
-  shows "set P' \<turnstile> lhs \<Rightarrow>* rhs"
+  assumes "trans1Tm A t G G'"
+    and "set (prods G) \<turnstile> lhs \<Rightarrow> rhs"
+  shows "set (prods G') \<turnstile> lhs \<Rightarrow>* rhs"
 proof -
-  obtain p' s' u v where "lhs = p'@[Nt u]@s' \<and> rhs = p'@v@s' \<and> (u,v) \<in> set P" (is "?uv")
+  obtain p' s' u v where "lhs = p'@[Nt u]@s' \<and> rhs = p'@v@s' \<and> (u,v) \<in> set (prods G)" (is "?uv")
     using assms(2) derive.cases by meson
-  obtain l r p s where "(l,r) \<in> set P \<and> (r = p@[Tm t]@s) \<and> (p \<noteq> [] \<or> s \<noteq> []) \<and> (A \<notin> Nts (set P))
-      \<and> set P' = ((set P - {(l,r)}) \<union> {(A,[Tm t]), (l, p@[Nt A]@s)})" (is "?lrps")
+  obtain l r p s where "(l,r) \<in> set (prods G) \<and> (r = p@[Tm t]@s) \<and> (p \<noteq> [] \<or> s \<noteq> []) \<and> (A \<notin> Nts (set (prods G)))
+      \<and> set (prods G') = ((set (prods G) - {(l,r)}) \<union> {(A,[Tm t]), (l, p@[Nt A]@s)})" (is "?lrps")
     using assms(1) set_removeAll fresh unfolding trans1Tm_def by fastforce
   thus ?thesis 
   proof (cases "u = l")
@@ -142,11 +211,11 @@ proof -
     then show ?thesis
     proof (cases "v = p@[Tm t]@s")
       case True
-      have 1: "(set P') \<turnstile> [Nt l] \<Rightarrow> p@[Nt A]@s"
+      have 1: "(set (prods G')) \<turnstile> [Nt l] \<Rightarrow> p@[Nt A]@s"
         using \<open>?lrps\<close> by (simp add: derive_singleton)
-      have "(set P') \<turnstile> [Nt A] \<Rightarrow> [Tm t]"
+      have "(set (prods G')) \<turnstile> [Nt A] \<Rightarrow> [Tm t]"
         using \<open>?lrps\<close> by (simp add: derive_singleton)
-      hence "(set P') \<turnstile> [Nt l] \<Rightarrow>* p@[Tm t]@s"
+      hence "(set (prods G')) \<turnstile> [Nt l] \<Rightarrow>* p@[Tm t]@s"
         using 1 by (meson converse_rtranclp_into_rtranclp r_into_rtranclp derive_append derive_prepend)
       thus ?thesis 
         using True \<open>u = l\<close> \<open>?uv\<close> derives_append derives_prepend by blast
@@ -163,14 +232,14 @@ proof -
 qed
 
 lemma cnf_r1Nt:
-  assumes "trans2Nt A B\<^sub>1 B\<^sub>2 P P'"
-    and "(set P) \<turnstile> lhs \<Rightarrow> rhs"
-  shows "(set P') \<turnstile> lhs \<Rightarrow>* rhs"
+  assumes "trans2Nt A B\<^sub>1 B\<^sub>2 G G'"
+    and "(set (prods G)) \<turnstile> lhs \<Rightarrow> rhs"
+  shows "(set (prods G')) \<turnstile> lhs \<Rightarrow>* rhs"
 proof -
-  obtain p' s' u v where "lhs = p'@[Nt u]@s' \<and> rhs = p'@v@s' \<and> (u,v) \<in> set P" (is "?uv")
+  obtain p' s' u v where "lhs = p'@[Nt u]@s' \<and> rhs = p'@v@s' \<and> (u,v) \<in> set (prods G)" (is "?uv")
     using assms(2) derive.cases by meson
-  obtain l r p s where "(l,r) \<in> set P \<and> (r = p@[Nt B\<^sub>1,Nt B\<^sub>2]@s) \<and> (p \<noteq> [] \<or> s \<noteq> []) \<and> (A \<notin> Nts (set P))
-    \<and> (set P' = ((set P - {(l,r)}) \<union> {(A, [Nt B\<^sub>1,Nt B\<^sub>2]), (l, p@[Nt A]@s)}))" (is "?lrps")
+  obtain l r p s where "(l,r) \<in> set (prods G) \<and> (r = p@[Nt B\<^sub>1,Nt B\<^sub>2]@s) \<and> (p \<noteq> [] \<or> s \<noteq> []) \<and> (A \<notin> Nts (set (prods G)))
+    \<and> (set (prods G') = ((set (prods G) - {(l,r)}) \<union> {(A, [Nt B\<^sub>1,Nt B\<^sub>2]), (l, p@[Nt A]@s)}))" (is "?lrps")
     using assms(1) set_removeAll fresh unfolding trans2Nt_def by fastforce
   thus ?thesis
   proof (cases "u = l")
@@ -178,11 +247,11 @@ proof -
     then show ?thesis 
     proof (cases "v = p@[Nt B\<^sub>1,Nt B\<^sub>2]@s")
       case True
-      have 1: "set P' \<turnstile> [Nt l] \<Rightarrow> p@[Nt A]@s"
+      have 1: "set (prods G') \<turnstile> [Nt l] \<Rightarrow> p@[Nt A]@s"
         using \<open>?lrps\<close> by (simp add: derive_singleton)
-      have "set P' \<turnstile> [Nt A] \<Rightarrow> [Nt B\<^sub>1,Nt B\<^sub>2]"
+      have "set (prods G') \<turnstile> [Nt A] \<Rightarrow> [Nt B\<^sub>1,Nt B\<^sub>2]"
         using \<open>?lrps\<close> by (simp add: derive_singleton)
-      hence "set P' \<turnstile> [Nt l] \<Rightarrow>* p@[Nt B\<^sub>1,Nt B\<^sub>2]@s" 
+      hence "set (prods G') \<turnstile> [Nt l] \<Rightarrow>* p@[Nt B\<^sub>1,Nt B\<^sub>2]@s" 
         using 1 by (meson converse_rtranclp_into_rtranclp derives_append derives_prepend r_into_rtranclp) 
       thus ?thesis 
         using True \<open>u = l\<close> \<open>?uv\<close> derives_append derives_prepend by blast
@@ -204,30 +273,30 @@ fun elim :: "('n, 't) prod \<Rightarrow> ('n, 't) syms \<Rightarrow> ('n, 't) sy
   "elim (A,\<alpha>) (r#rhs) = (if r = Nt A then \<alpha>@(elim (A,\<alpha>) rhs) else r#(elim (A,\<alpha>) rhs))"
 
 lemma slemma1_1: 
-  assumes "trans1Tm A t P P'"
-    and "(A, \<alpha>) \<in> set P'"
+  assumes "trans1Tm A t G G'"
+    and "(A, \<alpha>) \<in> set (prods G')"
   shows "\<alpha> = [Tm t]"
 proof -
-  have "A \<notin> Nts (set P)"
+  have "A \<notin> Nts (set (prods G))"
     using assms(1) fresh unfolding trans1Tm_def by blast
-  hence "\<nexists>\<alpha>. (A, \<alpha>) \<in> set P"
+  hence "\<nexists>\<alpha>. (A, \<alpha>) \<in> set (prods G)"
     unfolding Nts_def by auto
-  hence "\<nexists>\<alpha>. \<alpha> \<noteq> [Tm t] \<and> (A, \<alpha>) \<in> set P'"
+  hence "\<nexists>\<alpha>. \<alpha> \<noteq> [Tm t] \<and> (A, \<alpha>) \<in> set (prods G')"
     using assms(1) unfolding trans1Tm_def by auto
   thus ?thesis 
     using assms(2) by blast
 qed
 
 lemma slemma1_1Nt:
-  assumes "trans2Nt A B\<^sub>1 B\<^sub>2 P P'"
-    and "(A, \<alpha>) \<in> set P'"
+  assumes "trans2Nt A B\<^sub>1 B\<^sub>2 G G'"
+    and "(A, \<alpha>) \<in> set (prods G')"
   shows "\<alpha> = [Nt B\<^sub>1,Nt B\<^sub>2]"
 proof -
-  have "A \<notin> Nts (set P)"
+  have "A \<notin> Nts (set (prods G))"
     using assms(1) fresh unfolding trans2Nt_def by blast
-  hence "\<nexists>\<alpha>. (A, \<alpha>) \<in> set P"
+  hence "\<nexists>\<alpha>. (A, \<alpha>) \<in> set (prods G)"
     unfolding Nts_def  by auto
-  hence "\<nexists>\<alpha>. \<alpha> \<noteq> [Nt B\<^sub>1,Nt B\<^sub>2] \<and> (A, \<alpha>) \<in> set P'"
+  hence "\<nexists>\<alpha>. \<alpha> \<noteq> [Nt B\<^sub>1,Nt B\<^sub>2] \<and> (A, \<alpha>) \<in> set (prods G')"
     using assms(1) unfolding trans2Nt_def by auto
   thus ?thesis 
     using assms(2) by blast
@@ -254,46 +323,42 @@ lemma slemma4_3_1:
   shows "(\<alpha> = elim (A, \<alpha>) [Nt lhs])"
   using assms by simp
 
-lemma Nts_correct: "A \<notin> Nts P \<Longrightarrow> (\<nexists>S \<alpha>. (S, \<alpha>) \<in> P \<and> (Nt A \<in> {Nt S} \<union> set \<alpha>))"
-  unfolding Nts_def apply (induction rule: nt.induct) apply auto
-  by (metis Un_iff case_prod_conv in_set_conv_decomp insertCI nt.simps(2) nt_append)
-
 lemma slemma4_4:
-  assumes "trans1Tm A t P P'"
-    and "(l,r) \<in> set P"
+  assumes "trans1Tm A t G G'"
+    and "(l,r) \<in> set (prods G)"
   shows "(Nt A) \<notin> set r"
 proof -
-  have "A \<notin> Nts (set P)"
+  have "A \<notin> Nts (set (prods G))"
     using assms(1) fresh unfolding trans1Tm_def by blast
-  hence "\<nexists>S \<alpha>. (S, \<alpha>) \<in> set P \<and> (Nt A \<in> {Nt S} \<union> set \<alpha>)"
-    using Nts_correct[of A \<open>set P\<close>] by blast
+  hence "\<nexists>S \<alpha>. (S, \<alpha>) \<in> set (prods G) \<and> (Nt A \<in> {Nt S} \<union> set \<alpha>)"
+    using Nts_correct[of A \<open>set (prods G)\<close>] by blast
   thus ?thesis 
     using assms(2) by blast
 qed
 
 lemma slemma4_4Nt:
-  assumes "trans2Nt A B\<^sub>1 B\<^sub>2 P P'"
-    and "(l,r) \<in> set P"
+  assumes "trans2Nt A B\<^sub>1 B\<^sub>2 G G'"
+    and "(l,r) \<in> set (prods G)"
   shows "(Nt A) \<notin> set r"
 proof -
-  have "A \<notin> Nts (set P)"
+  have "A \<notin> Nts (set (prods G))"
     using assms(1) fresh unfolding trans2Nt_def by blast
-  hence "\<nexists>S \<alpha>. (S, \<alpha>) \<in> set P \<and> (Nt A \<in> {Nt S} \<union> set \<alpha>)"
-    using Nts_correct[of A \<open>set P\<close>] by blast
+  hence "\<nexists>S \<alpha>. (S, \<alpha>) \<in> set (prods G) \<and> (Nt A \<in> {Nt S} \<union> set \<alpha>)"
+    using Nts_correct[of A \<open>set (prods G)\<close>] by blast
   thus ?thesis 
     using assms(2) by blast
 qed
 
 
 lemma lemma1:
-  assumes "trans1Tm A t P P'"
-    and "set P' \<turnstile> lhs \<Rightarrow> rhs"
-  shows "(elim (A, [Tm t]) lhs = elim (A, [Tm t]) rhs) \<or> (set P \<turnstile> (elim (A, [Tm t]) lhs) \<Rightarrow> (elim (A, [Tm t]) rhs))"
+  assumes "trans1Tm A t G G'"
+    and "set (prods G') \<turnstile> lhs \<Rightarrow> rhs"
+  shows "(elim (A, [Tm t]) lhs = elim (A, [Tm t]) rhs) \<or> (set (prods G) \<turnstile> (elim (A, [Tm t]) lhs) \<Rightarrow> (elim (A, [Tm t]) rhs))"
 proof -
-  obtain l r p s where "(l,r) \<in> set P \<and> (r = p@[Tm t]@s) \<and> (p \<noteq> [] \<or> s \<noteq> []) \<and> (A \<notin> Nts (set P)) 
-      \<and> set P' = ((set P - {(l,r)}) \<union> {(A,[Tm t]), (l, p@[Nt A]@s)})" (is "?lrps")
+  obtain l r p s where "(l,r) \<in> set (prods G) \<and> (r = p@[Tm t]@s) \<and> (p \<noteq> [] \<or> s \<noteq> []) \<and> (A \<notin> Nts (set (prods G))) 
+      \<and> set (prods G') = ((set (prods G) - {(l,r)}) \<union> {(A,[Tm t]), (l, p@[Nt A]@s)})" (is "?lrps")
     using assms(1) set_removeAll fresh unfolding trans1Tm_def by fastforce
-  obtain p' s' u v where "lhs = p'@[Nt u]@s' \<and> rhs = p'@v@s' \<and> (u,v) \<in> set P'" (is "?uv")
+  obtain p' s' u v where "lhs = p'@[Nt u]@s' \<and> rhs = p'@v@s' \<and> (u,v) \<in> set (prods G')" (is "?uv")
     using assms(2) derive.cases by meson
   thus ?thesis
   proof (cases "u = A")
@@ -323,7 +388,7 @@ proof -
         using slemma4_0 by fast
       hence "elim (A, [Tm t]) v = p @ [Tm t] @ s"
         using 1 slemma4_0 slemma4_1 slemma4_3_1 by metis
-      hence 2: "(u, elim (A, [Tm t]) v) \<in> set P" using \<open>?lrps\<close> 
+      hence 2: "(u, elim (A, [Tm t]) v) \<in> set (prods G)" using \<open>?lrps\<close> 
         using True \<open>?uv\<close> assms(1) slemma4_4 by fastforce
       have "elim (A, [Tm t]) lhs = elim (A, [Tm t]) p' @ elim (A, [Tm t]) ([Nt u]@s')"
         using \<open>?uv\<close> slemma4_0 by fast
@@ -337,7 +402,7 @@ proof -
         using 2 3 assms(2) \<open>?uv\<close> derive.simps by fast
     next
       case False
-      hence 1: "(u, v) \<in> set P" 
+      hence 1: "(u, v) \<in> set (prods G)" 
         using assms(1) \<open>?uv\<close> \<open>u \<noteq> A\<close> \<open>?lrps\<close> by (simp add: in_set_conv_decomp)
        have "elim (A, [Tm t]) lhs = elim (A, [Tm t]) p' @ elim (A, [Tm t]) ([Nt u]@s')"
          using \<open>?uv\<close> slemma4_0 by fast
@@ -356,15 +421,15 @@ proof -
 qed
 
 lemma lemma1Nt: 
-  assumes "trans2Nt A B\<^sub>1 B\<^sub>2 P P'"
-    and "set P' \<turnstile> lhs \<Rightarrow> rhs"
+  assumes "trans2Nt A B\<^sub>1 B\<^sub>2 G G'"
+    and "set (prods G') \<turnstile> lhs \<Rightarrow> rhs"
   shows "(elim (A, [Nt B\<^sub>1,Nt B\<^sub>2]) lhs = elim (A, [Nt B\<^sub>1,Nt B\<^sub>2]) rhs) 
-          \<or> ((set P) \<turnstile> (elim (A, [Nt B\<^sub>1,Nt B\<^sub>2]) lhs) \<Rightarrow> elim (A, [Nt B\<^sub>1,Nt B\<^sub>2]) rhs)"
+          \<or> ((set (prods G)) \<turnstile> (elim (A, [Nt B\<^sub>1,Nt B\<^sub>2]) lhs) \<Rightarrow> elim (A, [Nt B\<^sub>1,Nt B\<^sub>2]) rhs)"
 proof -
-  obtain l r p s where "(l,r) \<in> set P \<and> (r = p@[Nt B\<^sub>1,Nt B\<^sub>2]@s) \<and> (p \<noteq> [] \<or> s \<noteq> []) \<and> (A \<notin> Nts (set P))
-    \<and> (set P' = ((set P - {(l,r)}) \<union> {(A, [Nt B\<^sub>1,Nt B\<^sub>2]), (l, p@[Nt A]@s)}))" (is "?lrps")
+  obtain l r p s where "(l,r) \<in> set (prods G) \<and> (r = p@[Nt B\<^sub>1,Nt B\<^sub>2]@s) \<and> (p \<noteq> [] \<or> s \<noteq> []) \<and> (A \<notin> Nts (set (prods G)))
+    \<and> (set (prods G') = ((set (prods G) - {(l,r)}) \<union> {(A, [Nt B\<^sub>1,Nt B\<^sub>2]), (l, p@[Nt A]@s)}))" (is "?lrps")
     using assms(1) set_removeAll fresh unfolding trans2Nt_def by fastforce
-  obtain p' s' u v where "lhs = p'@[Nt u]@s' \<and> rhs = p'@v@s' \<and> (u,v) \<in> set P'" (is "?uv")
+  obtain p' s' u v where "lhs = p'@[Nt u]@s' \<and> rhs = p'@v@s' \<and> (u,v) \<in> set (prods G')" (is "?uv")
     using assms(2) derive.cases by meson
   thus ?thesis
   proof (cases "u = A")
@@ -379,7 +444,7 @@ proof -
       have "elim (A, [Nt B\<^sub>1,Nt B\<^sub>2]) rhs = elim (A, [Nt B\<^sub>1,Nt B\<^sub>2]) p' @ elim (A, [Nt B\<^sub>1,Nt B\<^sub>2]) ([Nt B\<^sub>1,Nt B\<^sub>2]@s')"
         using \<open>?uv\<close> \<open>u = A\<close> slemma4_0 True by fast
       hence "elim (A, [Nt B\<^sub>1,Nt B\<^sub>2]) rhs = elim (A, [Nt B\<^sub>1,Nt B\<^sub>2]) p' @ [Nt B\<^sub>1,Nt B\<^sub>2] @ elim (A, [Nt B\<^sub>1,Nt B\<^sub>2]) s'"
-        using assms(1) trans2Nt_aux1[of A B\<^sub>1 B\<^sub>2 P P'] by fastforce 
+        using assms(1) trans2Nt_aux1[of A B\<^sub>1 B\<^sub>2 G G'] by fastforce 
       then show ?thesis
         using 1 by simp
     next
@@ -395,12 +460,12 @@ proof -
       have "Nt A \<notin> set p \<and> Nt A \<notin> set s" 
         using \<open>?lrps\<close> assms(1) by (metis UnI1 UnI2 set_append slemma4_4Nt)
       hence 1: "v = p@[Nt A]@s \<and> Nt A \<notin> set p \<and> Nt A \<notin> set s" 
-        using True \<open>?lrps\<close> \<open>?uv\<close> assms slemma4_4Nt[of A B\<^sub>1 B\<^sub>2 P P'] trans2Nt_aux1[of A B\<^sub>1 B\<^sub>2 P P'] by auto
+        using True \<open>?lrps\<close> \<open>?uv\<close> assms slemma4_4Nt[of A B\<^sub>1 B\<^sub>2 G G'] trans2Nt_aux1[of A B\<^sub>1 B\<^sub>2 G G'] by auto
       hence "elim (A, [Nt B\<^sub>1,Nt B\<^sub>2]) v = elim (A, [Nt B\<^sub>1,Nt B\<^sub>2]) p @ elim (A, [Nt B\<^sub>1,Nt B\<^sub>2]) ([Nt A]@s)"
         using slemma4_0 by fast
       hence "elim (A, [Nt B\<^sub>1,Nt B\<^sub>2]) v = p @ [Nt B\<^sub>1,Nt B\<^sub>2] @ s"
         using 1 slemma4_0 slemma4_1 slemma4_3_1 by metis
-      hence 2: "(u, elim (A, [Nt B\<^sub>1,Nt B\<^sub>2]) v) \<in> set P" 
+      hence 2: "(u, elim (A, [Nt B\<^sub>1,Nt B\<^sub>2]) v) \<in> set (prods G)" 
         using True \<open>?lrps\<close>  \<open>?uv\<close> assms(1) slemma4_4Nt by fastforce
       have "elim (A, [Nt B\<^sub>1,Nt B\<^sub>2]) lhs = elim (A, [Nt B\<^sub>1,Nt B\<^sub>2]) p' @ elim (A, [Nt B\<^sub>1,Nt B\<^sub>2]) ([Nt u]@s')"
         using \<open>?uv\<close> slemma4_0 by fast
@@ -414,7 +479,7 @@ proof -
         using 2 3 assms(2) \<open>?uv\<close> derive.simps by fast
     next
       case False
-      hence 1: "(u, v) \<in> set P" 
+      hence 1: "(u, v) \<in> set (prods G)" 
         using assms(1) \<open>?uv\<close> \<open>u \<noteq> A\<close> \<open>?lrps\<close> by (simp add: in_set_conv_decomp)
        have "elim (A, [Nt B\<^sub>1,Nt B\<^sub>2]) lhs = elim (A, [Nt B\<^sub>1,Nt B\<^sub>2]) p' @ elim (A, [Nt B\<^sub>1,Nt B\<^sub>2]) ([Nt u]@s')"
          using \<open>?uv\<close> slemma4_0 by fast
@@ -433,157 +498,157 @@ proof -
 qed
 
 lemma lemma3:
-  assumes "set P' \<turnstile> lhs \<Rightarrow>* rhs"
-    and "trans1Tm A t P P'"
-  shows "set P \<turnstile> (elim (A, [Tm t]) lhs) \<Rightarrow>* (elim (A, [Tm t]) rhs)"
+  assumes "set (prods G') \<turnstile> lhs \<Rightarrow>* rhs"
+    and "trans1Tm A t G G'"
+  shows "set (prods G) \<turnstile> (elim (A, [Tm t]) lhs) \<Rightarrow>* (elim (A, [Tm t]) rhs)"
   using assms
 proof (induction)
   case (step y z)
   then show ?case 
-    using lemma1[of A t P P' y z] rtranclp.rtrancl_into_rtrancl by fastforce 
+    using lemma1[of A t G G' y z] rtranclp.rtrancl_into_rtrancl by fastforce 
 qed simp
 
 lemma lemma3Nt:
-  assumes "set P' \<turnstile> lhs \<Rightarrow>* rhs"
-    and "trans2Nt A B\<^sub>1 B\<^sub>2 P P'"
-  shows "set P \<turnstile> (elim (A, [Nt B\<^sub>1, Nt B\<^sub>2]) lhs) \<Rightarrow>* (elim (A, [Nt B\<^sub>1, Nt B\<^sub>2]) rhs)"
+  assumes "set (prods G') \<turnstile> lhs \<Rightarrow>* rhs"
+    and "trans2Nt A B\<^sub>1 B\<^sub>2 G G'"
+  shows "set (prods G) \<turnstile> (elim (A, [Nt B\<^sub>1, Nt B\<^sub>2]) lhs) \<Rightarrow>* (elim (A, [Nt B\<^sub>1, Nt B\<^sub>2]) rhs)"
   using assms 
 proof (induction)
   case (step y z)
   then show ?case 
-    using lemma1Nt[of A B\<^sub>1 B\<^sub>2 P P' y z] rtranclp.rtrancl_into_rtrancl by fastforce 
+    using lemma1Nt[of A B\<^sub>1 B\<^sub>2 G G' y z] rtranclp.rtrancl_into_rtrancl by fastforce 
 qed simp
 
 lemma slemma4_7: "map Tm w = elim (A, \<alpha>) (map Tm w)"
   by (induction w) auto
 
 lemma slemma4_2: 
-  assumes "trans1Tm A t P P'"
-    and "N \<in> Nts (set P)"
+  assumes "trans1Tm A t G G'"
+    and "N \<in> Nts (set (prods G))"
   shows "[Nt N] = elim (A, [Tm t]) [Nt N]"
   using assms fresh unfolding trans1Tm_def by auto
 
 lemma slemma4_2Nt: 
-  assumes "trans2Nt A B\<^sub>1 B\<^sub>2 P P'"
-    and "N \<in> Nts (set P)"
+  assumes "trans2Nt A B\<^sub>1 B\<^sub>2 G G'"
+    and "N \<in> Nts (set (prods G))"
   shows "[Nt N] = elim (A, [Nt B\<^sub>1, Nt B\<^sub>2]) [Nt N]"
   using assms fresh unfolding trans2Nt_def by auto
 
 lemma lemma4:
-  assumes "trans1Tm A t P P'" 
-    and "S \<in> Nts (set P)"
-  shows "lang P' S \<subseteq> lang P S"
+  assumes "trans1Tm A t G G'" 
+  shows "L G' \<subseteq> L G"
 proof 
   fix w
-  assume "w \<in> lang P' S"
-  hence "set P' \<turnstile> [Nt S] \<Rightarrow>* map Tm w"
+  assume "w \<in> L G'"
+  hence "set (prods G') \<turnstile> [Nt (start G')] \<Rightarrow>* map Tm w"
     unfolding Lang_def by simp
-  hence "set P' \<turnstile> [Nt S] \<Rightarrow>* map Tm w"
+  hence "set (prods G') \<turnstile> [Nt (start G)] \<Rightarrow>* map Tm w"
     using assms unfolding trans1Tm_def by auto
-  hence "set P \<turnstile> elim (A, [Tm t]) [Nt S] \<Rightarrow>*  elim (A, [Tm t]) (map Tm w)"
-    using assms lemma3[of P' \<open>[Nt S]\<close> \<open>map Tm w\<close> A t P] by blast
-  moreover have "elim (A, [Tm t]) [Nt S] = [Nt S]"
-    using assms fresh unfolding trans1Tm_def by auto
+  hence "set (prods G) \<turnstile> elim (A, [Tm t]) [Nt (start G)] \<Rightarrow>*  elim (A, [Tm t]) (map Tm w)"
+    using assms lemma3[of G' \<open>[Nt (start G)]\<close> \<open>map Tm w\<close> A t G] by blast
+  moreover have "elim (A, [Tm t]) [Nt (start G)] = [Nt (start G)]"
+    using assms fresh unfolding trans1Tm_def 
+    by (metis Un_iff singletonI slemma4_2_0 slemma4_2_1) (*TODO*)
   moreover have "elim (A, [Tm t]) (map Tm w) = map Tm w" 
-    using \<open>w \<in> lang P' S\<close> slemma4_7 by metis
-  ultimately show "w \<in> lang P S" 
-    using L_def \<open>w \<in> lang P' S\<close> by (simp add: Lang_def)
+    using \<open>w \<in> L G'\<close> slemma4_7 by metis
+  ultimately show "w \<in> L G" 
+    using  \<open>w \<in> L G'\<close> by (simp add: Lang_def)
 qed
 
 lemma lemma4Nt:
-  assumes "trans2Nt A B\<^sub>1 B\<^sub>2 P P'"
-    and "S \<in> Nts (set P)"
-  shows "lang P' S \<subseteq> lang P S"
+  assumes "trans2Nt A B\<^sub>1 B\<^sub>2 G G'"
+  shows "L G' \<subseteq> L G"
 proof
   fix w
-  assume "w \<in> lang P' S"
-  hence "set P' \<turnstile> [Nt S] \<Rightarrow>* map Tm w"
+  assume "w \<in> L G'"
+  hence "set (prods G') \<turnstile> [Nt (start G')] \<Rightarrow>* map Tm w"
     by (simp add: Lang_def)
-  hence "set P' \<turnstile> [Nt S] \<Rightarrow>* map Tm w"
+  hence "set (prods G') \<turnstile> [Nt (start G)] \<Rightarrow>* map Tm w"
     using assms unfolding trans2Nt_def by auto
-  hence "set P \<turnstile> elim (A, [Nt B\<^sub>1, Nt B\<^sub>2]) [Nt S] \<Rightarrow>*  elim (A, [Nt B\<^sub>1, Nt B\<^sub>2]) (map Tm w)"
-    using assms lemma3Nt[of P' \<open>[Nt S]\<close> \<open>map Tm w\<close> A B\<^sub>1 B\<^sub>2 P] by blast
-  moreover have "elim (A, [Nt B\<^sub>1, Nt B\<^sub>2]) [Nt S] = [Nt S]"
-    using assms fresh unfolding trans2Nt_def by auto 
+  hence "set (prods G) \<turnstile> elim (A, [Nt B\<^sub>1, Nt B\<^sub>2]) [Nt (start G)] \<Rightarrow>*  elim (A, [Nt B\<^sub>1, Nt B\<^sub>2]) (map Tm w)"
+    using assms lemma3Nt[of G' \<open>[Nt (start G)]\<close> \<open>map Tm w\<close> A B\<^sub>1 B\<^sub>2 G] by blast
+  moreover have "elim (A, [Nt B\<^sub>1, Nt B\<^sub>2]) [Nt (start G)] = [Nt (start G)]"
+    using assms fresh unfolding trans2Nt_def 
+    by (metis UnCI singletonI slemma4_2_0 slemma4_2_1) (*TODO*)
   moreover have "elim (A, [Nt B\<^sub>1, Nt B\<^sub>2]) (map Tm w) = map Tm w" 
-    using \<open>w \<in> lang P' S\<close> slemma4_7 by metis
-  ultimately show "w \<in> lang P S" using Lang_def \<open>w \<in> lang P' S\<close> 
+    using \<open>w \<in> L G'\<close> slemma4_7 by metis
+  ultimately show "w \<in> L G" using Lang_def \<open>w \<in> L G'\<close> 
     by (metis (no_types, lifting) mem_Collect_eq)
 qed
 
 lemma slemma5_1:
-  assumes "set P \<turnstile> lhs \<Rightarrow>* rhs"
+  assumes "set (prods G) \<turnstile> lhs \<Rightarrow>* rhs"
     and "lhs = [Nt S]"
-    and "trans1Tm A t P P'"
-  shows "set P' \<turnstile> lhs \<Rightarrow>* rhs"
+    and "trans1Tm A t G G'"
+  shows "set (prods G') \<turnstile> lhs \<Rightarrow>* rhs"
   using assms apply (induction) apply auto by (meson cnf_r1Tm rtranclp_trans)
 
 lemma slemma5_1Nt:
-  assumes "set P \<turnstile> lhs \<Rightarrow>* rhs"
+  assumes "set (prods G) \<turnstile> lhs \<Rightarrow>* rhs"
     and "lhs = [Nt S]"
-    and "trans2Nt A B\<^sub>1 B\<^sub>2 P P'"
-  shows "set P' \<turnstile> lhs \<Rightarrow>* rhs"
+    and "trans2Nt A B\<^sub>1 B\<^sub>2 G G'"
+  shows "set (prods G') \<turnstile> lhs \<Rightarrow>* rhs"
   using assms apply (induction) apply auto by (meson cnf_r1Nt rtranclp_trans)
 
 lemma lemma5: 
-  assumes "trans1Tm A t P P'"
-  shows "lang P S \<subseteq> lang P' S"
+  assumes "trans1Tm A t G G'"
+  shows "L G \<subseteq> L G'"
 proof 
   fix w
-  assume "w \<in> lang P S"
-  hence "set P \<turnstile> [Nt S] \<Rightarrow>* map Tm w"
-    unfolding Lang_def by simp
-  thus "w \<in> lang P' S" 
+  assume "w \<in> L G"
+  hence "set (prods G) \<turnstile> [Nt (start G')] \<Rightarrow>* map Tm w"
+    using assms unfolding Lang_def trans1Tm_def by auto 
+  thus "w \<in> L G'" 
     using assms slemma5_1 Lang_def by fastforce
 qed 
 
 lemma lemma5Nt: 
-  assumes "trans2Nt A B\<^sub>1 B\<^sub>2 P P'"
-  shows "lang P S \<subseteq> lang P' S"
+  assumes "trans2Nt A B\<^sub>1 B\<^sub>2 G G'"
+  shows "L G \<subseteq> L G'"
 proof 
   fix w
-  assume "w \<in> lang P S"
-  hence "set P \<turnstile> [Nt S] \<Rightarrow>* map Tm w"
-    unfolding Lang_def by simp
-  thus "w \<in> lang P' S" 
+  assume "w \<in> L G"
+  hence "set (prods G) \<turnstile> [Nt (start G')] \<Rightarrow>* map Tm w"
+    using assms unfolding Lang_def trans2Nt_def by auto 
+  thus "w \<in> L G'" 
     using assms slemma5_1Nt Lang_def by fast
 qed 
 
 lemma cnf_lemma1: 
-  assumes "trans1Tm A t P P'" "S \<in> Nts (set P)"
-  shows "lang P S = lang P' S"
+  assumes "trans1Tm A t G G'"
+  shows "L G = L G'"
   using assms lemma4 lemma5 by fast
 
 lemma cnf_lemma1Nt: 
-  assumes "trans2Nt A B\<^sub>1 B\<^sub>2 P P'" "S \<in> Nts (set P)"
-  shows "lang P S = lang P' S"
+  assumes "trans2Nt A B\<^sub>1 B\<^sub>2 G G'"
+  shows "L G = L G'"
   using assms lemma4Nt lemma5Nt by fast
 
-definition eqLang :: "('n,'t) prods \<Rightarrow> ('n,'t) prods \<Rightarrow> 'n \<Rightarrow> bool" where
-  "eqLang P P' S \<longleftrightarrow> lang P S = lang P' S"
+definition eqLang :: "('n,'t) cfg \<Rightarrow> ('n,'t) cfg \<Rightarrow> bool" where
+  "eqLang G G' \<longleftrightarrow> L G = L G'"
 
 lemma trans1TmRtc_noeProds: 
-  assumes "((\<lambda>x y. \<exists>A t. trans1Tm A t x y) ^**) P P'"
-    and "noeProds (set P)"
-  shows "noeProds (set P')"
+  assumes "((\<lambda>x y. \<exists>A t. trans1Tm A t x y) ^**) G G'"
+    and "noeProds (set (prods G))"
+  shows "noeProds (set (prods G'))"
   using assms by (induction) (auto simp: trans1Tm_noeProds)
 
 lemma trans2NtRtc_noeProds:
-  assumes "((\<lambda>x y. \<exists>A t B\<^sub>1 B\<^sub>2. trans2Nt A B\<^sub>1 B\<^sub>2 x y) ^**) P P'"
-    and "noeProds (set P)"
-  shows "noeProds (set P')"
+  assumes "((\<lambda>x y. \<exists>A t B\<^sub>1 B\<^sub>2. trans2Nt A B\<^sub>1 B\<^sub>2 x y) ^**) G G'"
+    and "noeProds (set (prods G))"
+  shows "noeProds (set (prods G'))"
   using assms by (induction) (auto simp: trans2Nt_noeProds)
 
 lemma trans1TmRtc_noUnitProds: 
-  assumes "((\<lambda>x y. \<exists>A t. trans1Tm A t x y) ^**) P P'"
-    and "noUnitProds (set P)"
-  shows "noUnitProds (set P')"
+  assumes "((\<lambda>x y. \<exists>A t. trans1Tm A t x y) ^**) G G'"
+    and "noUnitProds (set (prods G))"
+  shows "noUnitProds (set (prods G'))"
   using assms by (induction) (auto simp: trans1Tm_noUnitProds)
 
 lemma trans2NtRtc_noUnitProds:
-  assumes "((\<lambda>x y. \<exists>A t B\<^sub>1 B\<^sub>2. trans2Nt A B\<^sub>1 B\<^sub>2 x y) ^**) P P'"
-    and "noUnitProds (set P)"
-  shows "noUnitProds (set P')"
+  assumes "((\<lambda>x y. \<exists>A t B\<^sub>1 B\<^sub>2. trans2Nt A B\<^sub>1 B\<^sub>2 x y) ^**) G G'"
+    and "noUnitProds (set (prods G))"
+  shows "noUnitProds (set (prods G'))"
   using assms by (induction) (auto simp: trans2Nt_noUnitProds)
 
 (* proofs about Nts and an arbitrary start Symbol S *)
@@ -592,11 +657,11 @@ lemma Nts_aux1: "Nts (P \<union> P') = Nts P \<union> Nts P'"
   unfolding Nts_def by simp
 
 lemma trans1Tm_Nts: 
-  assumes "trans1Tm A t P P'" "S \<in> Nts (set P)"
-  shows "S \<in> Nts (set P')"
+  assumes "trans1Tm A t G G'" "S \<in> Nts (set (prods G))"
+  shows "S \<in> Nts (set (prods G'))"
 proof -
-  obtain l r p s where "(l,r) \<in> set P \<and> (r = p@[Tm t]@s) \<and> (p \<noteq> [] \<or> s \<noteq> []) \<and> (A \<notin> Nts (set P)) 
-      \<and> set P' = ((set P - {(l,r)}) \<union> {(A,[Tm t]), (l, p@[Nt A]@s)})" (is "?lrps")
+  obtain l r p s where "(l,r) \<in> set (prods G) \<and> (r = p@[Tm t]@s) \<and> (p \<noteq> [] \<or> s \<noteq> []) \<and> (A \<notin> Nts (set (prods G))) 
+      \<and> set (prods G') = ((set (prods G) - {(l,r)}) \<union> {(A,[Tm t]), (l, p@[Nt A]@s)})" (is "?lrps")
     using assms(1) set_removeAll fresh unfolding trans1Tm_def by fastforce
   thus ?thesis
   proof (cases "S \<in> Nts {(l,r)}")
@@ -606,7 +671,7 @@ proof -
     then show ?thesis using  \<open>?lrps\<close> Nts_aux1 by (metis UnCI)
   next
     case False
-    hence "S \<in> Nts (set P - {(l,r)})"
+    hence "S \<in> Nts (set (prods G) - {(l,r)})"
       unfolding Nts_def using \<open>?lrps\<close> 
       by (metis UnCI UnE Un_Diff_cancel2 assms(2) Nts_aux1 Nts_def)
     then show ?thesis 
@@ -615,16 +680,16 @@ proof -
 qed  
 
 lemma trans1TmRtc_Nts: 
-  assumes "((\<lambda>x y. \<exists>A t. trans1Tm A t x y) ^**) P P'" "S \<in> Nts (set P)"
-  shows "S \<in> Nts (set P')"
+  assumes "((\<lambda>x y. \<exists>A t. trans1Tm A t x y) ^**) G G'" "S \<in> Nts (set (prods G))"
+  shows "S \<in> Nts (set (prods G'))"
   using assms by (induction rule: rtranclp.induct) (auto simp: trans1Tm_Nts)
 
 lemma trans2Nt_Nts: 
-  assumes "trans2Nt A B\<^sub>1 B\<^sub>2 P P'" "S \<in> Nts (set P)"
-  shows "S \<in> Nts (set P')"
+  assumes "trans2Nt A B\<^sub>1 B\<^sub>2 G G'" "S \<in> Nts (set (prods G))"
+  shows "S \<in> Nts (set (prods G'))"
 proof -
-  obtain l r p s where "(l,r) \<in> set P \<and> (r = p@[Nt B\<^sub>1,Nt B\<^sub>2]@s) \<and> (p \<noteq> [] \<or> s \<noteq> []) \<and> (A \<notin> Nts (set P))
-    \<and> (set P' = ((set P - {(l,r)}) \<union> {(A, [Nt B\<^sub>1,Nt B\<^sub>2]), (l, p@[Nt A]@s)}))" (is "?lrps")
+  obtain l r p s where "(l,r) \<in> set (prods G) \<and> (r = p@[Nt B\<^sub>1,Nt B\<^sub>2]@s) \<and> (p \<noteq> [] \<or> s \<noteq> []) \<and> (A \<notin> Nts (set (prods G)))
+    \<and> (set (prods G') = ((set (prods G) - {(l,r)}) \<union> {(A, [Nt B\<^sub>1,Nt B\<^sub>2]), (l, p@[Nt A]@s)}))" (is "?lrps")
     using assms(1) set_removeAll fresh unfolding trans2Nt_def by fastforce
     thus ?thesis
   proof (cases "S \<in> Nts {(l,r)}")
@@ -635,7 +700,7 @@ proof -
       using  \<open>?lrps\<close> Nts_aux1 by (metis UnCI)
   next
     case False
-    hence "S \<in> Nts (set P - {(l,r)})"
+    hence "S \<in> Nts (set (prods G) - {(l,r)})"
       unfolding Nts_def using \<open>?lrps\<close> 
       by (metis UnCI UnE Un_Diff_cancel2 assms(2) Nts_aux1 Nts_def)
     then show ?thesis 
@@ -644,27 +709,26 @@ proof -
 qed  
 
 lemma trans2NtRtc_Nts: 
-  assumes "((\<lambda>x y. \<exists>A t B\<^sub>1 B\<^sub>2. trans2Nt A B\<^sub>1 B\<^sub>2 x y) ^**) P P'" "S \<in> Nts (set P)"
-  shows "S \<in> Nts (set P')"
+  assumes "((\<lambda>x y. \<exists>A t B\<^sub>1 B\<^sub>2. trans2Nt A B\<^sub>1 B\<^sub>2 x y) ^**) G G'" "S \<in> Nts (set (prods G))"
+  shows "S \<in> Nts (set (prods G'))"
   using assms by (induction rule: rtranclp.induct) (auto simp: trans2Nt_Nts)
 
 (* Termination for an arbitrary start Symbol S *)
 
 theorem cnf_lemma2: 
-  assumes "((\<lambda>x y. \<exists>A t. trans1Tm A t x y) ^**) P P'" "S \<in> Nts (set P)" 
-  shows "(lang P S = lang P' S)"
-  using assms by (induction rule: rtranclp.induct) (fastforce simp: cnf_lemma1 trans1TmRtc_Nts)+
+  assumes "((\<lambda>x y. \<exists>A t. trans1Tm A t x y) ^**) G G'"
+  shows "L G = L G'"
+  using assms by (induction rule: rtranclp.induct) (fastforce simp: cnf_lemma1)+ 
 
 theorem cnf_lemma2Nt: 
-  assumes "((\<lambda>x y. \<exists>A B\<^sub>1 B\<^sub>2. trans2Nt A B\<^sub>1 B\<^sub>2 x y) ^**) P P'" "S \<in> Nts (set P)" 
-  shows "(lang P S = lang P' S)"
-  using assms by (induction rule: rtranclp.induct) (fastforce simp: cnf_lemma1Nt trans2NtRtc_Nts)+
+  assumes "((\<lambda>x y. \<exists>A t B\<^sub>1 B\<^sub>2. trans2Nt A B\<^sub>1 B\<^sub>2 x y) ^**) G G'"
+  shows "L G = L G'"
+  using assms by (induction rule: rtranclp.induct) (fastforce simp: cnf_lemma1Nt)+
 
 theorem cnf_lemma: 
-  assumes "((\<lambda>x y. \<exists>A t. trans1Tm A t x y) ^**) P P'"
-    and "((\<lambda>x y. \<exists>A B\<^sub>1 B\<^sub>2. trans2Nt A B\<^sub>1 B\<^sub>2 x y) ^**) P' P''"
-    and "S \<in> Nts (set P)"
-  shows "lang P S = lang P'' S"
+  assumes "((\<lambda>x y. \<exists>A t. trans1Tm A t x y) ^**) G G'"
+    and "((\<lambda>x y. \<exists>A B\<^sub>1 B\<^sub>2. trans2Nt A B\<^sub>1 B\<^sub>2 x y) ^**) G' G''"
+  shows "L G = L G''"
   using assms cnf_lemma2 cnf_lemma2Nt trans1TmRtc_Nts by fastforce
 
 (* Part 2 *)
@@ -695,96 +759,96 @@ lemma badNtsCount_removeAll2:
   using assms by (induction P) fastforce+
 
 lemma lemma6_a: 
-  assumes "trans1Tm A t P P'" 
-  shows "badTmsCount P' < badTmsCount P"
+  assumes "trans1Tm A t G G'" 
+  shows "badTmsCount (prods G') < badTmsCount (prods G)"
 proof -
-  obtain l r p s where "(l,r) \<in> set P \<and> (r = p@[Tm t]@s) \<and> (p \<noteq> [] \<or> s \<noteq> []) \<and> (A \<notin> Nts (set P)) 
-      \<and> P' = ((removeAll (l,r) P) @ [(A,[Tm t]), (l, p@[Nt A]@s)])" (is "?lrps")
+  obtain l r p s where "(l,r) \<in> set (prods G) \<and> (r = p@[Tm t]@s) \<and> (p \<noteq> [] \<or> s \<noteq> []) \<and> (A \<notin> Nts (set (prods G))) 
+      \<and> prods G' = ((removeAll (l,r) (prods G)) @ [(A,[Tm t]), (l, p@[Nt A]@s)])" (is "?lrps")
     using assms fresh unfolding trans1Tm_def by auto
   hence "prodTms (l,p@[Tm t]@s) = length (filter (isTmnlSym) (p@[Tm t]@s))"
     unfolding prodTms_def by auto
   hence 1: "prodTms (l,p@[Tm t]@s) = Suc (length (filter (isTmnlSym) (p@s)))"
     by (simp add: isTmnlSym_def)
-  have 2: "badTmsCount P' = badTmsCount (removeAll (l,r) P) + badTmsCount [(A,[Tm t])] + badTmsCount [(l, p@[Nt A]@s)]"
+  have 2: "badTmsCount (prods G') = badTmsCount (removeAll (l,r) (prods G)) + badTmsCount [(A,[Tm t])] + badTmsCount [(l, p@[Nt A]@s)]"
     using \<open>?lrps\<close> by (auto simp: badTmsCount_append)
-  have 3: "badTmsCount (removeAll (l,r) P) < badTmsCount P"
+  have 3: "badTmsCount (removeAll (l,r) (prods G)) < badTmsCount (prods G)"
     using 1 badTmsCount_removeAll \<open>?lrps\<close> gr0_conv_Suc by blast
   have "prodTms (l, p@[Nt A]@s) = (length (filter (isTmnlSym) (p@[Nt A]@s))) \<or> prodTms (l, p@[Nt A]@s) = 0"
     unfolding prodTms_def using \<open>?lrps\<close> by simp
   thus ?thesis
   proof 
     assume "prodTms (l, p@[Nt A]@s) = (length (filter (isTmnlSym) (p@[Nt A]@s)))"
-    hence "badTmsCount P' = badTmsCount (removeAll (l,r) P) + prodTms (l, p@[Nt A]@s)"
+    hence "badTmsCount (prods G') = badTmsCount (removeAll (l,r) (prods G)) + prodTms (l, p@[Nt A]@s)"
       using 2 by (simp add: prodTms_def)
     moreover have "prodTms (l,p@[Nt A]@s) < prodTms (l,p@[Tm t]@s)"
       using 1 \<open>prodTms (l, p @ [Nt A] @ s) = length (filter isTmnlSym (p @ [Nt A] @ s))\<close> isTmnlSym_def by force 
-    ultimately show "badTmsCount P' < badTmsCount P" 
-      using badTmsCount_removeAll2[of "(l,r)" P "(l,p @[Nt A]@s)"] \<open>?lrps\<close> 1 by auto
+    ultimately show "badTmsCount (prods G') < badTmsCount (prods G)" 
+      using badTmsCount_removeAll2[of "(l,r)" "prods G" "(l,p @[Nt A]@s)"] \<open>?lrps\<close> 1 by auto
   next 
     assume "prodTms (l, p@[Nt A]@s) = 0"
-    hence "badTmsCount P' = badTmsCount (removeAll (l,r) P)"
+    hence "badTmsCount (prods G') = badTmsCount (removeAll (l,r) (prods G))"
       using 2 by (simp add: prodTms_def)
-    thus "badTmsCount P' < badTmsCount P" 
+    thus "badTmsCount (prods G') < badTmsCount (prods G)" 
       using 3 by simp
   qed
 qed
 
 lemma lemma6_b: 
-  assumes "trans2Nt A B\<^sub>1 B\<^sub>2 P P'"
-  shows "badNtsCount P' < badNtsCount P"
+  assumes "trans2Nt A B\<^sub>1 B\<^sub>2 G G'"
+  shows "badNtsCount (prods G') < badNtsCount (prods G)"
 proof -
-  obtain l r p s where "(l,r) \<in> set P \<and> (r = p@[Nt B\<^sub>1,Nt B\<^sub>2]@s) \<and> (p \<noteq> [] \<or> s \<noteq> []) \<and> (A \<notin> Nts (set P))
-    \<and> (P' = ((removeAll (l,r) P) @ [(A, [Nt B\<^sub>1,Nt B\<^sub>2]), (l, p@[Nt A]@s)]))" (is "?lrps")
+  obtain l r p s where "(l,r) \<in> set (prods G) \<and> (r = p@[Nt B\<^sub>1,Nt B\<^sub>2]@s) \<and> (p \<noteq> [] \<or> s \<noteq> []) \<and> (A \<notin> Nts (set (prods G)))
+    \<and> prods G' = ((removeAll (l,r) (prods G)) @ [(A, [Nt B\<^sub>1,Nt B\<^sub>2]), (l, p@[Nt A]@s)])" (is "?lrps")
     using assms(1) fresh unfolding trans2Nt_def by auto
   hence "prodNts (l,p@[Nt B\<^sub>1,Nt B\<^sub>2]@s) = length (filter (isNonTmnlSym) (p@[Nt B\<^sub>1,Nt B\<^sub>2]@s))"
     unfolding prodNts_def by auto
   hence 1: "prodNts (l,p@[Nt B\<^sub>1,Nt B\<^sub>2]@s) = Suc (Suc (length (filter (isNonTmnlSym) (p@s))))"
     by (simp add: isNonTmnlSym_def)
-  have 2: "badNtsCount P' = badNtsCount (removeAll (l,r) P) + badNtsCount [(A, [Nt B\<^sub>1,Nt B\<^sub>2])] + badNtsCount [(l, (p@[Nt A]@s))]"
+  have 2: "badNtsCount (prods G') = badNtsCount (removeAll (l,r) (prods G)) + badNtsCount [(A, [Nt B\<^sub>1,Nt B\<^sub>2])] + badNtsCount [(l, (p@[Nt A]@s))]"
     using \<open>?lrps\<close> by (auto simp: badNtsCount_append prodNts_def)
-  have 3: "badNtsCount (removeAll (l,r) P) < badNtsCount P"
+  have 3: "badNtsCount (removeAll (l,r) (prods G)) < badNtsCount (prods G)"
     using \<open>?lrps\<close> badNtsCount_removeAll 1 by force
   have "prodNts (l, p@[Nt A]@s) = length (filter (isNonTmnlSym) (p@[Nt A]@s)) \<or> prodNts (l, p@[Nt A]@s) = 0"
     unfolding prodNts_def using \<open>?lrps\<close> by simp
   thus ?thesis 
   proof 
     assume "prodNts (l, p@[Nt A]@s) = length (filter (isNonTmnlSym) (p@[Nt A]@s))"
-    hence "badNtsCount P' = badNtsCount (removeAll (l,r) P) + badNtsCount [(l, (p@[Nt A]@s))]"
+    hence "badNtsCount (prods G') = badNtsCount (removeAll (l,r) (prods G)) + badNtsCount [(l, (p@[Nt A]@s))]"
       using 2 by (simp add: prodNts_def)
     moreover have "prodNts (l, p@[Nt A]@s) < prodNts (l,p@[Nt B\<^sub>1,Nt B\<^sub>2]@s)"
       using 1 \<open>prodNts (l, p@[Nt A]@s) = length (filter (isNonTmnlSym) (p@[Nt A]@s))\<close> isNonTmnlSym_def by simp
     ultimately show ?thesis 
-      using badNtsCount_removeAll2[of "(l,r)" P "(l, (p@[Nt A]@s))"] 1 \<open>?lrps\<close> by auto
+      using badNtsCount_removeAll2[of "(l,r)" "prods G" "(l, (p@[Nt A]@s))"] 1 \<open>?lrps\<close> by auto
   next 
     assume "prodNts (l, p@[Nt A]@s) = 0"
-    hence "badNtsCount P' = badNtsCount (removeAll (l,r) P)"
+    hence "badNtsCount (prods G') = badNtsCount (removeAll (l,r) (prods G))"
       using 2 by (simp add: prodNts_def)
     thus ?thesis 
       using 3 by simp
   qed
 qed
 
-lemma lemma7_a: "trans1Tm A t P P' \<Longrightarrow> badTmsCount P > 0"
+lemma lemma7_a: "trans1Tm A t G G' \<Longrightarrow> badTmsCount (prods G) > 0"
   using lemma6_a by fastforce
 
-lemma lemma7_b: "trans2Nt A B\<^sub>1 B\<^sub>2 P P' \<Longrightarrow> badNtsCount P > 0"
+lemma lemma7_b: "trans2Nt A B\<^sub>1 B\<^sub>2 G G' \<Longrightarrow> badNtsCount (prods G) > 0"
   using lemma6_b by fastforce
 
 lemma badTmsCount0_removeAll: "badTmsCount P = 0 \<Longrightarrow> badTmsCount (removeAll (l,r) P) = 0" 
   by (induction P) auto 
 
 lemma slemma15_a:
-  assumes "trans2Nt A B\<^sub>1 B\<^sub>2 P P'"
-    and "badTmsCount P = 0"
-  shows "badTmsCount P' = 0"
+  assumes "trans2Nt A B\<^sub>1 B\<^sub>2 G G'"
+    and "badTmsCount (prods G) = 0"
+  shows "badTmsCount (prods G') = 0"
 proof -
-  obtain l r p s where "(l,r) \<in> set P \<and> (r = p@[Nt B\<^sub>1,Nt B\<^sub>2]@s) \<and> (p \<noteq> [] \<or> s \<noteq> []) \<and> (A \<notin> Nts (set P))
-    \<and> (P' = ((removeAll (l,r) P) @ [(A, [Nt B\<^sub>1,Nt B\<^sub>2]), (l, p@[Nt A]@s)]))" (is "?lrps")
+  obtain l r p s where "(l,r) \<in> set (prods G) \<and> (r = p@[Nt B\<^sub>1,Nt B\<^sub>2]@s) \<and> (p \<noteq> [] \<or> s \<noteq> []) \<and> (A \<notin> Nts (set (prods G)))
+    \<and> (prods G' = ((removeAll (l,r) (prods G)) @ [(A, [Nt B\<^sub>1,Nt B\<^sub>2]), (l, p@[Nt A]@s)]))" (is "?lrps")
     using assms(1) fresh unfolding trans2Nt_def by auto
-  hence "badTmsCount P' = badTmsCount (removeAll (l,r) P) + badTmsCount [(l, (p@[Nt A]@s))]"
+  hence "badTmsCount (prods G') = badTmsCount (removeAll (l,r) (prods G)) + badTmsCount [(l, (p@[Nt A]@s))]"
     by (auto simp: badTmsCount_append prodTms_def isTmnlSym_def)
-  moreover have "badTmsCount (removeAll (l,r) P) = 0"
-    using badTmsCount0_removeAll[of P l r] assms(2) by simp
+  moreover have "badTmsCount (removeAll (l,r) (prods G)) = 0"
+    using badTmsCount0_removeAll[of \<open>prods G\<close> l r] assms(2) by simp
   moreover have "badTmsCount [(l, (p@[Nt A]@s))] = 0" 
   proof -
     have "prodTms (l,p@[Nt B\<^sub>1,Nt B\<^sub>2]@s) = 0"
@@ -797,9 +861,9 @@ proof -
 qed
 
 lemma lemma15_a:
-  assumes "((\<lambda>x y. \<exists>A B\<^sub>1 B\<^sub>2. trans2Nt A B\<^sub>1 B\<^sub>2 x y) ^**) P P'"
-    and "badTmsCount P = 0"
-  shows "badTmsCount P' = 0"
+  assumes "((\<lambda>x y. \<exists>A B\<^sub>1 B\<^sub>2. trans2Nt A B\<^sub>1 B\<^sub>2 x y) ^**) G G'"
+    and "badTmsCount (prods G) = 0"
+  shows "badTmsCount (prods G') = 0"
   using assms by (induction) (auto simp: slemma15_a)
 
 lemma noTms_prodTms0:
@@ -813,12 +877,12 @@ proof -
 qed
 
 lemma badTmsCountNot0:
-  assumes "badTmsCount P > 0"
-  shows "\<exists>l r t. (l,r) \<in> set P \<and> length r \<ge> 2 \<and> Tm t \<in> set r"
+  assumes "badTmsCount (prods G) > 0"
+  shows "\<exists>l r t. (l,r) \<in> set (prods G) \<and> length r \<ge> 2 \<and> Tm t \<in> set r"
 proof -
-  have "\<exists>p \<in> set P. prodTms p > 0"
+  have "\<exists>p \<in> set (prods G). prodTms p > 0"
     using assms badTmsCountSet not_gr0 by blast
-  from this obtain l r where "(l, r) \<in> set P \<and> prodTms (l,r) > 0" (is "?lr")
+  from this obtain l r where "(l, r) \<in> set (prods G) \<and> prodTms (l,r) > 0" (is "?lr")
     by auto
   hence 1: "length r \<ge> 2"
     unfolding prodTms_def using not_le_imp_less by fastforce
@@ -830,12 +894,12 @@ proof -
 qed
 
 lemma badNtsCountNot0: 
-  assumes "badNtsCount P > 0" 
-  shows "\<exists>l r. (l, r) \<in> set P \<and> length r \<ge> 3"
+  assumes "badNtsCount (prods G) > 0" 
+  shows "\<exists>l r. (l, r) \<in> set (prods G) \<and> length r \<ge> 3"
 proof -
-  have "\<exists>p \<in> set P. prodNts p > 0"
+  have "\<exists>p \<in> set (prods G). prodNts p > 0"
     using assms badNtsCountSet not_gr0 by blast
-  from this obtain l r where "(l, r) \<in> set P \<and> prodNts (l,r) > 0" (is "?lr")
+  from this obtain l r where "(l, r) \<in> set (prods G) \<and> prodNts (l,r) > 0" (is "?lr")
     by auto
   hence "length r \<ge> 3"
     unfolding prodNts_def using not_le_imp_less by fastforce
@@ -849,108 +913,169 @@ lemma list_longer3: "length l \<ge> 3 \<Longrightarrow> (\<exists>hd tl x y. l =
   by (metis Suc_le_length_iff append.left_neutral append_Cons neq_Nil_conv numeral_3_eq_3)
 
 lemma lemma8_a:
-  assumes "badTmsCount P > 0"
-  shows "\<exists>P' A t. trans1Tm A t P P'"
+  assumes "badTmsCount (prods G) > 0"
+  shows "\<exists>G' A t. trans1Tm A t G G'"
 proof -
-  obtain l r t where "(l,r) \<in> set P \<and> length r \<ge> 2 \<and> Tm t \<in> set r" (is "?lr")
+  obtain l r t where "(l,r) \<in> set (prods G) \<and> length r \<ge> 2 \<and> Tm t \<in> set r" (is "?lr")
     using assms badTmsCountNot0 by blast
-  hence "\<exists>p s. r = p@[Tm t]@s \<and> (p \<noteq> [] \<or> s \<noteq> [])" 
+  from this obtain p s where "r = p@[Tm t]@s \<and> (p \<noteq> [] \<or> s \<noteq> [])" (is "?ps")
     unfolding isTmnlSym_def using \<open>?lr\<close> list_longer2[of r] by blast
-  thus ?thesis
-    unfolding trans1Tm_def using \<open>?lr\<close> by blast
+  from this obtain A G' where "A = fresh G \<and> G' = cfg (removeAll (l, r) (prods G) @ [(A, [Tm t]), (l, p @ [Nt A] @ s)]) (start G)" 
+    by auto
+  hence "trans1Tm A t G G'"
+    unfolding trans1Tm_def using \<open>?lr\<close>  \<open>?ps\<close> by auto
+  thus ?thesis by blast
 qed
 
+thm trans2Nt_def
 lemma lemma8_b:
-  assumes "badTmsCount P = 0"
-    and "badNtsCount P > 0"
-  shows "\<exists>P' A B\<^sub>1 B\<^sub>2. trans2Nt A B\<^sub>1 B\<^sub>2 P P'"
+  assumes "badTmsCount (prods G) = 0"
+    and "badNtsCount (prods G) > 0"
+  shows "\<exists>G' A B\<^sub>1 B\<^sub>2. trans2Nt A B\<^sub>1 B\<^sub>2 G G'"
 proof -
-  obtain l r where "(l, r) \<in> set P \<and> length r \<ge> 3" (is "?lr")
+  obtain l r where "(l, r) \<in> set (prods G) \<and> length r \<ge> 3" (is "?lr")
     using assms(2) badNtsCountNot0 by blast
   obtain p s X Y where "r = p@[X]@[Y]@s \<and> (p \<noteq> [] \<or> s \<noteq> [])" (is "?psXY")
     using \<open>?lr\<close> list_longer3[of r] by blast
   have "(\<forall>a \<in> set r. isNonTmnlSym a)"
-    using \<open>?lr\<close> assms(1) badTmsCountSet[of P] noTms_prodTms0[of l r] by simp
-  hence "\<exists>B\<^sub>1 B\<^sub>2. X = Nt B\<^sub>1 \<and> Y = Nt B\<^sub>2"
-    using isNonTmnlSym_def \<open>?psXY\<close> by auto
-  hence "\<exists>B\<^sub>1 B\<^sub>2. (r = p@[Nt B\<^sub>1,Nt B\<^sub>2]@s) \<and> (p \<noteq> [] \<or> s \<noteq> [])"
+    using \<open>?lr\<close> assms(1) badTmsCountSet[of \<open>prods G\<close>] noTms_prodTms0[of l r] by simp
+  from this obtain B\<^sub>1 B\<^sub>2 where "X = Nt B\<^sub>1 \<and> Y = Nt B\<^sub>2"
+    using isNonTmnlSym_def \<open>?psXY\<close> by fastforce
+  hence "(r = p@[Nt B\<^sub>1,Nt B\<^sub>2]@s) \<and> (p \<noteq> [] \<or> s \<noteq> [])" (is "?B")
     using \<open>?psXY\<close> by auto
-  thus ?thesis
-    using trans2Nt_def \<open>?lr\<close> by blast
+  from this obtain A G' where "A = fresh G \<and> G' = cfg (removeAll (l, r) (prods G) @ [(A, [Nt B\<^sub>1, Nt B\<^sub>2]), (l, p @ [Nt A] @ s)]) (start G)"
+    by simp
+  hence "trans2Nt A B\<^sub>1 B\<^sub>2 G G'"
+    unfolding trans2Nt_def using \<open>?lr\<close> \<open>?B\<close> by auto
+  thus ?thesis by blast
 qed
 
-lemma lemma11_a: "\<nexists>P' A t. trans1Tm A t P P' \<Longrightarrow> badTmsCount P = 0"
+lemma lemma11_a: "\<nexists>G' A t. trans1Tm A t G G' \<Longrightarrow> badTmsCount (prods G) = 0"
   using lemma8_a by blast
 
 lemma lemma11_b: 
-  assumes "\<nexists>P' A B\<^sub>1 B\<^sub>2. trans2Nt A B\<^sub>1 B\<^sub>2 P P'"
-    and "badTmsCount P = 0" 
-    shows "badNtsCount P = 0"
+  assumes "\<nexists>G' A B\<^sub>1 B\<^sub>2. trans2Nt A B\<^sub>1 B\<^sub>2 G G'"
+    and "badTmsCount (prods G) = 0" 
+    shows "badNtsCount (prods G) = 0"
   using assms lemma8_b by blast
 
-thm converse_rtranclp_into_rtranclp
-lemma trans1Tm_2: "\<exists>P'. ((\<lambda>x y. \<exists>A t. trans1Tm A t x y) ^**) P P' \<and> (badTmsCount P' = 0)"
-proof (induction "badTmsCount P" arbitrary: P rule: less_induct)
+lemma trans1Tm_2: "\<exists>G'. ((\<lambda>x y. \<exists>A t. trans1Tm A t x y) ^**) G G' \<and> (badTmsCount (prods G') = 0)"
+proof (induction "badTmsCount (prods G)" arbitrary: G rule: less_induct)
   case less
   then show ?case
-  proof (cases "badTmsCount P = 0")
+  proof (cases "badTmsCount (prods G) = 0")
     case False
-    from this obtain P' A t where "trans1Tm A t P P'" (is "?P'")
+    from this obtain G' A t where "trans1Tm A t G G'" (is "?G'")
       using lemma8_a by blast
-    hence "badTmsCount P' < badTmsCount P"
-      using lemma6_a[of A t P P'] by blast
-    from this obtain P'' where "(\<lambda>x y. \<exists>A t. trans1Tm A t x y)\<^sup>*\<^sup>* P' P'' \<and> badTmsCount P'' = 0"
+    hence "badTmsCount (prods G') < badTmsCount (prods G)"
+      using lemma6_a[of A t G G'] by blast
+    from this obtain G'' where "(\<lambda>x y. \<exists>A t. trans1Tm A t x y)\<^sup>*\<^sup>* G' G'' \<and> badTmsCount (prods G'') = 0"
       using less by blast
     thus ?thesis 
-      using \<open>?P'\<close> converse_rtranclp_into_rtranclp[of "(\<lambda>x y. \<exists>A t. trans1Tm A t x y)" P P' P''] by blast
+      using \<open>?G'\<close> converse_rtranclp_into_rtranclp[of "(\<lambda>x y. \<exists>A t. trans1Tm A t x y)" G G' G''] by blast
   qed blast
 qed
 
-thm lemma11_b lemma6_b slemma15_a converse_rtranclp_into_rtranclp rtranclp.rtrancl_refl
 lemma trans2Nt_2: 
-  assumes "badTmsCount P = 0"
-    shows "\<exists>P'. ((\<lambda>x y. \<exists>A B\<^sub>1 B\<^sub>2. trans2Nt A B\<^sub>1 B\<^sub>2 x y) ^**) P P' \<and> (badNtsCount P' = 0)"
-using assms proof (induction "badNtsCount P" arbitrary: P rule: less_induct)
+  assumes "badTmsCount (prods G) = 0"
+    shows "\<exists>G'. ((\<lambda>x y. \<exists>A B\<^sub>1 B\<^sub>2. trans2Nt A B\<^sub>1 B\<^sub>2 x y) ^**) G G' \<and> (badNtsCount (prods G') = 0)"
+using assms proof (induction "badNtsCount (prods G)" arbitrary: G rule: less_induct)
   case less
   then show ?case 
-  proof (cases "badNtsCount P = 0")
+  proof (cases "badNtsCount (prods G) = 0")
     case False
-    from this obtain P' A B\<^sub>1 B\<^sub>2 where "trans2Nt A B\<^sub>1 B\<^sub>2 P P'" (is "?P'")
+    from this obtain G' A B\<^sub>1 B\<^sub>2 where "trans2Nt A B\<^sub>1 B\<^sub>2 G G'" (is "?G'")
       using assms lemma8_b less(2) by blast
-    hence "badNtsCount P' < badNtsCount P"
+    hence "badNtsCount (prods G') < badNtsCount (prods G)"
       using lemma6_b by blast
-    from this obtain P'' where "(\<lambda>x y. \<exists>A B\<^sub>1 B\<^sub>2. trans2Nt A B\<^sub>1 B\<^sub>2 x y)\<^sup>*\<^sup>* P' P'' \<and> badNtsCount P'' = 0"
-      using less slemma15_a[of A B\<^sub>1 B\<^sub>2 P P'] \<open>?P'\<close> by blast
+    from this obtain G'' where "(\<lambda>x y. \<exists>A B\<^sub>1 B\<^sub>2. trans2Nt A B\<^sub>1 B\<^sub>2 x y)\<^sup>*\<^sup>* G' G'' \<and> badNtsCount (prods G'') = 0"
+      using less slemma15_a[of A B\<^sub>1 B\<^sub>2 G G'] \<open>?G'\<close> by blast
     then show ?thesis 
-      using \<open>?P'\<close> converse_rtranclp_into_rtranclp[of "(\<lambda>x y. \<exists>A B\<^sub>1 B\<^sub>2. trans2Nt A B\<^sub>1 B\<^sub>2 x y)" P P' P''] by blast
+      using \<open>?G'\<close> converse_rtranclp_into_rtranclp[of "(\<lambda>x y. \<exists>A B\<^sub>1 B\<^sub>2. trans2Nt A B\<^sub>1 B\<^sub>2 x y)" G G' G''] by blast
   qed blast
 qed
 
-theorem thm4_5: "S \<in> Nts (set (P::('n::infinite,'t) prods)) \<Longrightarrow> \<exists>P'. (cnf P') \<and> (lang P S = lang P' S)"
-proof -
-  obtain P' where "((\<lambda>x y. \<exists>A t. trans1Tm A t x y) ^**) P P' \<and> (badTmsCount P' = 0)" (is "?P'")
+theorem thm4_5: "\<forall>G::('n::infinite,'t) cfg. \<exists>G'::('n,'t)cfg. cnf G' \<and> L G = L G'"
+proof 
+  fix G::"('n::infinite,'t) cfg"
+  obtain G' where "((\<lambda>x y. \<exists>A t. trans1Tm A t x y) ^**) G G' \<and> (badTmsCount (prods G') = 0)" (is "?G'")
     using trans1Tm_2 by blast
-  obtain P'' where "((\<lambda>x y. \<exists>A B\<^sub>1 B\<^sub>2. trans2Nt A B\<^sub>1 B\<^sub>2 x y) ^**) P' P'' \<and> (badNtsCount P'' = 0) \<and> (badTmsCount P'' = 0)" (is "?P''")
-    using \<open>?P'\<close> trans2Nt_2 lemma15_a by blast
-  hence "cnf P''"
+  obtain G'' where "((\<lambda>x y. \<exists>A B\<^sub>1 B\<^sub>2. trans2Nt A B\<^sub>1 B\<^sub>2 x y) ^**) G' G'' \<and> (badNtsCount (prods G'') = 0) \<and> (badTmsCount (prods G'') = 0)" (is "?G''")
+    using \<open>?G'\<close> trans2Nt_2 lemma15_a by blast
+  hence "cnf G''"
     using cnf_def by blast
-  moreover have "S \<in> Nts (set P) \<Longrightarrow> lang P S = lang P'' S"
-    using \<open>?P'\<close> \<open>?P''\<close> cnf_lemma by blast
-  ultimately show "S \<in> Nts (set P) \<Longrightarrow> \<exists>P'. (cnf P') \<and> (lang P S = lang P' S)" 
-    using \<open>?P'\<close> \<open>?P''\<close> by blast
+  moreover have "L G = L G''"
+    using \<open>?G'\<close> \<open>?G''\<close> cnf_lemma by blast
+  ultimately show "\<exists>G'::('n,'t)cfg. cnf G' \<and> L G = L G'"
+    by blast
 qed
 
-definition "isCnf P \<equiv> (\<forall>l r. (l,r) \<in> set P \<longrightarrow> (
+theorem cnf_noe_noUnit: 
+  assumes "noeProds (set (prods (G::('n::infinite,'t) cfg)))" "noUnitProds (set (prods G))"
+  shows "\<exists>G'::('n,'t) cfg. (cnf G') \<and> (L G = L G') \<and> noeProds (set (prods G')) \<and> noUnitProds (set (prods G'))"
+proof -
+  obtain G' where "((\<lambda>x y. \<exists>A t. trans1Tm A t x y) ^**) G G' \<and> (badTmsCount (prods G') = 0) \<and> noeProds (set (prods G')) \<and> noUnitProds (set (prods G'))" (is "?G'")
+    using assms trans1Tm_2 trans1TmRtc_noeProds trans1TmRtc_noUnitProds by blast
+  obtain G'' where "((\<lambda>x y. \<exists>A B\<^sub>1 B\<^sub>2. trans2Nt A B\<^sub>1 B\<^sub>2 x y) ^**) G' G'' \<and> (badNtsCount (prods G'') = 0) \<and> (badTmsCount (prods G'') = 0)" (is "?G''")
+    using \<open>?G'\<close> trans2Nt_2 lemma15_a by blast
+  hence "cnf G'' \<and> noeProds (set (prods G'')) \<and> noUnitProds (set (prods G''))"
+    using \<open>?G'\<close> cnf_def trans2NtRtc_noeProds trans2NtRtc_noUnitProds by fastforce
+  moreover have "L G = L G''"
+    using \<open>?G'\<close> \<open>?G''\<close> cnf_lemma by blast
+  ultimately show ?thesis
+    using \<open>?G'\<close> \<open>?G''\<close> assms(1) by blast
+qed
+
+
+definition isCnf :: "('n, 't) cfg \<Rightarrow> bool" where
+  "isCnf G \<equiv> (\<forall>(l,r) \<in> set (prods G).
     (length r = 2 \<and> list_all (isNonTmnlSym) r) \<or> 
-    (length r = 1 \<and> list_all (isTmnlSym) r)))"
+    (length r = 1 \<and> list_all (isTmnlSym) r))"
+
+lemma isCnf_eq_cnf: "isCnf G \<longleftrightarrow> (cnf G \<and> noeProds (set (prods G)) \<and> noUnitProds (set (prods G)))"
+proof 
+  assume "isCnf G" (is "?assm")
+  hence "noeProds (set (prods G))"
+    unfolding isCnf_def noeProds_def by fastforce
+  moreover have "noUnitProds (set (prods G))"
+    using \<open>?assm\<close> unfolding isCnf_def noUnitProds_def isNonTmnlSym_def isTmnlSym_def by fastforce
+  moreover have "cnf G"
+    using \<open>?assm\<close> unfolding isCnf_def cnf_def isNonTmnlSym_def isTmnlSym_def prodNts_def prodTms_def sorry
+  ultimately show "cnf G \<and> noeProds (set (prods G)) \<and> noUnitProds (set (prods G))"
+    by blast
+next 
+  assume "cnf G \<and> noeProds (set (prods G)) \<and> noUnitProds (set (prods G))" (is "?assm")
+  hence "binary G \<and> uniform G"
+    using cnf_bin_un by blast
+  hence "\<forall>(A, \<alpha>) \<in> set (prods G). length \<alpha> \<le> 2"
+    unfolding binary_def by simp
+  hence "\<forall>(A, \<alpha>) \<in> set (prods G). length \<alpha> = 2 \<or> length \<alpha> = 1"
+    using \<open>?assm\<close> nat_neq_iff unfolding noeProds_def by fastforce
+  thus "isCnf G"
+    unfolding noUnitProds_def isCnf_def sorry
+qed
 
 theorem cnf_exists: 
-  assumes "S \<in> Nts (set (P::('n::infinite,'t) prods))" 
-  shows "\<exists>P'. (isCnf P') \<and> (lang P' S = lang P S - {[]})"
-proof -
-  have "\<exists>P\<^sub>0. nepr P P\<^sub>0" 
+  shows "\<forall>G::('n::infinite,'t) cfg. \<exists>G'::('n,'t) cfg. (isCnf G') \<and> (L G' = L G - {[]})"
+proof
+  fix G::"('n,'t)cfg"
+  obtain P\<^sub>0 where "nepr (prods G) P\<^sub>0" (is "?P\<^sub>0")
     using nepr_exists by blast
-  thus ?thesis sorry
+  obtain P\<^sub>u where "uppr P\<^sub>0 P\<^sub>u" (is "?P\<^sub>u")
+    using uppr_exists by blast
+  obtain G\<^sub>u where "G\<^sub>u = cfg P\<^sub>u (start G)" (is "?G\<^sub>u")
+    by simp
+  hence 1: "noeProds (set (prods G\<^sub>u)) \<and> noUnitProds (set (prods G\<^sub>u))"
+    using \<open>?P\<^sub>0\<close> \<open>?P\<^sub>u\<close> negrImpnoeProds upgrImpnoUnitProds upgr_noeProds by fastforce
+  have 2: "L G\<^sub>u = L G - {[]}"
+    using \<open>?P\<^sub>0\<close> \<open>?P\<^sub>u\<close> \<open>?G\<^sub>u\<close> nepr_uppr_lang_eq[of \<open>prods G\<close> P\<^sub>0 P\<^sub>u \<open>start G\<close>] by (simp add: nepr_lang_eq)
+  obtain G'::"('n,'t) cfg" where "cnf G' \<and> L G\<^sub>u = L G' \<and> noeProds (set (prods G')) \<and> noUnitProds (set (prods G'))" (is "?G'")
+    using 1 cnf_noe_noUnit by blast
+  hence "isCnf G'" 
+    using \<open>?G'\<close> isCnf_eq_cnf by blast
+  moreover have "L G' = L G - {[]}"
+    using 2 \<open>?G'\<close> by blast
+  ultimately show "\<exists>G'::('n,'t) cfg. (isCnf G') \<and> (L G' = L G - {[]})" by blast
 qed
 
 end
